\documentclass[answers,12pt]{exam}
\oddsidemargin 0pt
\evensidemargin 0 pt
\topmargin -.4in
\headsep 20pt
\footskip 20pt
\textheight 8.8in
\textwidth 6.25in
\input{macros}
\usepackage{tikz}
\usetikzlibrary{shapes,arrows}
\usepackage{color}
\usepackage{answers}
\usepackage{amsmath}
\usepackage{amsfonts}
\usepackage{enumitem}
\usepackage{amsthm}
%\usepackage{booktabs}
\usepackage{graphicx}
\newcommand\tab[1][1cm]{\hspace*{#1}}
\shadedsolutions
\begin{document}
	\begin{flushright}Your name here\end{flushright}
		\section*{Lab 8: Proofs by Numerical Induction}
Note to reader: these aren't exactly the most \textbf{wordy} proofs - you should make yours wordier :).
\begin{questions}

%%%%%%%%%%%%%%%%%%%%%%%%

%%%Example 1%%%
\question[some]
For all natural numbers $n \geq 2$, $3^{n} > n^{2}$.

\begin{solution} \\
\textit{Claim.} For all natural numbers $n \geq 2, 3^n > n^2$ \\
		\begin{proof}(Induct on $n$.)\\
			Base Case ($n$ = 2):\\
			\tab $3^2 = 9 > 4 = 2^2$\\
			Induction Step:\\
			\tab Choose a $k \in \mathbb{N}$ with $k \geq 2$, and assume $3^k > k^2$\\
			\tab \tab \tab $3^{k+1} = 3 \cdot 3^k$\\
			\tab \tab \tab $> 3 \cdot k^2$ \hfill (by IH)\\
			\tab \tab \tab $= k^2 + k^2 + k^2$\\
			\tab \tab \tab $= k^2 + k \cdot k + k \cdot k$\\
			\tab \tab \tab $\geq k^2 + 2k + 2 \cdot 2$\hfill (since $k \geq 2$)\\
			\tab \tab \tab $= k^2 + 2k + 4$\\
			\tab \tab \tab $> k^2 + 2k + 1$\\
			\tab \tab \tab $= (k+1)^2$\\
			\tab Therefore $3^{k+1} > (k+1)^2$
		\end{proof}
\end{solution}
  
%%%Example 2%%%
\question[some]
For all natural numbers $n \geq 1$, $\displaystyle\sum_{i-1}^{n} 2^{i-1} = 2^{n} - 1$\\

\begin{solution} \\
	\textit{Claim.} For all natural numbers $n \geq 1$, $\displaystyle\sum_{i-1}^{n} 2^{i-1} = 2^{n} - 1$\\
		\begin{proof}(Induct on $n$.)\\
			Base Case ($n$ = 1):\\
			\tab $\displaystyle\sum_{i=1}^{1} 2^{1-1} = 1$, and $2^1 - 1 = 1$.\\
			\tab So therefore $\displaystyle\sum_{i=1}^{1} 2^{i-1} = 2^1 - 1$\\
			Inductive Step:\\
			\tab Assume that for some positive integer $k$, $\displaystyle\sum_{i=1}^{k} 2^{i-1} = 2^k - 1$\\
			\tab \tab \tab $\displaystyle\sum_{i=1}^{k+1} 2^{i-1} = \displaystyle\sum_{i=1}^{k} 2^{i-1} + 2^{k}$\\
			\tab \tab \tab $=2^k -1 + 2^k$\hfill (by IH)\\
			\tab \tab \tab $=2(2^k)-1$\\
			\tab \tab \tab $=2^{k+1}-1$\\
			\tab So $\displaystyle\sum_{i=1}^{k+1} 2^{i-1} = 2^{k+1} -1$
		\end{proof}
\end{solution}

%%%%%%%%%%%%%%%%%%%%%%%%%TODO%%%%%%%%%%%%%%%%%%%%%%%%%%%%%%%%%%%%%%%%%%%%%
\question[some]
For all natural numbers, $n \geq 7, 3^{n} < n!$.
		

\begin{solution}
	proof goes here
\end{solution}

%%%%%%%%%%%%%%%%%%%%%%%
\question[some] 
	For all natural numbers $n \geq 1, \displaystyle\sum_{i=1}^{n} 2i = n(n+1)$.


\begin{solution}
	proof goes here
\end{solution}

%%%%%%%%%%%%%%%%%%%%%%
\question[some]
	For all $n \in \mathbb{N}, n^{2} - 3n$ is even.


\begin{solution}
	this is a proof
\end{solution}
 
%%%%%%%%%%%%%%%%%%%%%
\end{questions}
\end{document}

